examples-c/linked-lists/has_cycle.c
@@ -1,6 +1,9 @@
 
 #include "list.h"
 
+/*@ logic Has_cycle_variant has_cycle_variant(list l, list l1, list l2)
+  reads l->tl */
+
 /*@ requires
   @   finite(l)
   @ ensures 
@@ -12,8 +15,8 @@ int cyclic(list l) {
   if (!l1) return 0;
   l2 = l1->tl;
   /*@ invariant (\exists plist pl1; lpath(l,pl1,l1)) &&
-    @           (\exists plist pl2; lpath(l,pl2,l2)) &&
-    @           (\exists plist pl12; lpath(l1,pl12,l2))
+    @           (\exists plist pl12; lpath(l1,pl12,l2) && pl12!=nil())
+    @ variant has_cycle_variant(l,l1,l2) for has_cycle_order
     @*/
   while (l1 != l2) {
     if (!l1 || !l2 || !l2->tl) return 0;
